src/Init/Data/UInt/Lemmas.lean
@@ -34,14 +34,22 @@ macro "declare_uint_theorems" typeName:ident bits:term:arg : command => do
   @[deprecated toNat_ofNatLT (since := "2025-02-13")]
   theorem toNat_ofNatCore {n : Nat} {h : n < size} : (ofNatLT n h).toNat = n := BitVec.toNat_ofNatLT ..
 
-  @[simp] theorem toFin_val_eq_toNat (x : $typeName) : x.toFin.val = x.toNat := rfl
-  @[deprecated toFin_val_eq_toNat (since := "2025-02-12")]
+  @[simp] theorem toFin_val (x : $typeName) : x.toFin.val = x.toNat := rfl
+  @[deprecated toFin_val (since := "2025-02-12")]
   theorem val_val_eq_toNat (x : $typeName) : x.toFin.val = x.toNat := rfl
 
+  @[simp] theorem toNat_toBitVec (x : $typeName) : x.toBitVec.toNat = x.toNat := rfl
+  @[simp] theorem toFin_toBitVec (x : $typeName) : x.toBitVec.toFin = x.toFin := rfl
+
+  @[deprecated toNat_toBitVec (since := "2025-02-21")]
   theorem toNat_toBitVec_eq_toNat (x : $typeName) : x.toBitVec.toNat = x.toNat := rfl
 
-  @[simp] theorem ofBitVec_toBitVec_eq : ∀ (a : $typeName), ofBitVec a.toBitVec = a
+  @[simp] theorem ofBitVec_toBitVec : ∀ (a : $typeName), ofBitVec a.toBitVec = a
     | ⟨_, _⟩ => rfl
+
+  @[deprecated ofBitVec_toBitVec (since := "2025-02-21")]
+  theorem ofBitVec_toBitVec_eq : ∀ (a : $typeName), ofBitVec a.toBitVec = a :=
+    ofBitVec_toBitVec
 
   @[deprecated ofBitVec_toBitVec_eq (since := "2025-02-12")]
   theorem mk_toBitVec_eq : ∀ (a : $typeName), ofBitVec a.toBitVec = a
@@ -241,21 +249,174 @@ declare_uint_theorems USize System.Platform.numBits
 
 @[simp] theorem USize.toNat_ofNat32 {n : Nat} {h : n < 4294967296} : (ofNat32 n h).toNat = n := rfl
 
-@[simp] theorem USize.toNat_toUInt32 (x : USize) : x.toUInt32.toNat = x.toNat % 2 ^ 32  := rfl
-
+@[simp] theorem USize.toNat_toUInt8 (x : USize) : x.toUInt8.toNat = x.toNat % 2 ^ 8 := rfl
+@[simp] theorem USize.toNat_toUInt16 (x : USize) : x.toUInt16.toNat = x.toNat % 2 ^ 16 := rfl
+@[simp] theorem USize.toNat_toUInt32 (x : USize) : x.toUInt32.toNat = x.toNat % 2 ^ 32 := rfl
 @[simp] theorem USize.toNat_toUInt64 (x : USize) : x.toUInt64.toNat = x.toNat := rfl
 
 theorem USize.toNat_ofNat_of_lt_32 {n : Nat} (h : n < 4294967296) : toNat (ofNat n) = n :=
-  toNat_ofNat_of_lt (Nat.lt_of_lt_of_le h le_usize_size)
+  toNat_ofNat_of_lt (Nat.lt_of_lt_of_le h USize.le_size)
 
 theorem UInt32.toNat_lt_of_lt {n : UInt32} {m : Nat} (h : m < size) : n < ofNat m → n.toNat < m := by
-  simp [lt_def, BitVec.lt_def, UInt32.toNat, toBitVec_eq_of_lt h]
+  simp [-toNat_toBitVec, lt_def, BitVec.lt_def, UInt32.toNat, toBitVec_eq_of_lt h]
 
 theorem UInt32.lt_toNat_of_lt {n : UInt32} {m : Nat} (h : m < size) : ofNat m < n → m < n.toNat := by
-  simp [lt_def, BitVec.lt_def, UInt32.toNat, toBitVec_eq_of_lt h]
+  simp [-toNat_toBitVec, lt_def, BitVec.lt_def, UInt32.toNat, toBitVec_eq_of_lt h]
 
 theorem UInt32.toNat_le_of_le {n : UInt32} {m : Nat} (h : m < size) : n ≤ ofNat m → n.toNat ≤ m := by
-  simp [le_def, BitVec.le_def, UInt32.toNat, toBitVec_eq_of_lt h]
+  simp [-toNat_toBitVec, le_def, BitVec.le_def, UInt32.toNat, toBitVec_eq_of_lt h]
 
 theorem UInt32.le_toNat_of_le {n : UInt32} {m : Nat} (h : m < size) : ofNat m ≤ n → m ≤ n.toNat := by
-  simp [le_def, BitVec.le_def, UInt32.toNat, toBitVec_eq_of_lt h]
+  simp [-toNat_toBitVec, le_def, BitVec.le_def, UInt32.toNat, toBitVec_eq_of_lt h]
+
+@[simp] theorem UInt8.toNat_lt (n : UInt8) : n.toNat < 2 ^ 8 := n.toFin.isLt
+@[simp] theorem UInt16.toNat_lt (n : UInt16) : n.toNat < 2 ^ 16 := n.toFin.isLt
+@[simp] theorem UInt32.toNat_lt (n : UInt32) : n.toNat < 2 ^ 32 := n.toFin.isLt
+@[simp] theorem UInt64.toNat_lt (n : UInt64) : n.toNat < 2 ^ 64 := n.toFin.isLt
+
+theorem UInt8.size_lt_usizeSize : UInt8.size < USize.size := by
+  cases USize.size_eq <;> simp_all +decide
+theorem UInt8.size_le_usizeSize : UInt8.size ≤ USize.size :=
+  Nat.le_of_lt UInt8.size_lt_usizeSize
+theorem UInt16.size_lt_usizeSize : UInt16.size < USize.size := by
+  cases USize.size_eq <;> simp_all +decide
+theorem UInt16.size_le_usizeSize : UInt16.size ≤ USize.size :=
+  Nat.le_of_lt UInt16.size_lt_usizeSize
+theorem UInt32.size_le_usizeSize : UInt32.size ≤ USize.size := by
+  cases USize.size_eq <;> simp_all +decide
+theorem USize.size_eq_two_pow : USize.size = 2 ^ System.Platform.numBits := rfl
+theorem USize.toNat_lt_two_pow_numBits (n : USize) : n.toNat < 2 ^ System.Platform.numBits := n.toFin.isLt
+@[simp] theorem USize.toNat_lt (n : USize) : n.toNat < 2 ^ 64 := Nat.lt_of_lt_of_le n.toFin.isLt size_le
+
+theorem UInt8.toNat_lt_usizeSize (n : UInt8) : n.toNat < USize.size :=
+  Nat.lt_of_lt_of_le n.toNat_lt (by cases USize.size_eq <;> simp_all)
+theorem UInt16.toNat_lt_usizeSize (n : UInt16) : n.toNat < USize.size :=
+  Nat.lt_of_lt_of_le n.toNat_lt (by cases USize.size_eq <;> simp_all)
+theorem UInt32.toNat_lt_usizeSize (n : UInt32) : n.toNat < USize.size :=
+  Nat.lt_of_lt_of_le n.toNat_lt (by cases USize.size_eq <;> simp_all)
+
+@[simp] theorem Fin.mk_uInt8ToNat (n : UInt8) : Fin.mk n.toNat n.toFin.isLt = n.toFin := rfl
+@[simp] theorem Fin.mk_uInt16ToNat (n : UInt16) : Fin.mk n.toNat n.toFin.isLt = n.toFin := rfl
+@[simp] theorem Fin.mk_uInt32ToNat (n : UInt32) : Fin.mk n.toNat n.toFin.isLt = n.toFin := rfl
+@[simp] theorem Fin.mk_uInt64ToNat (n : UInt64) : Fin.mk n.toNat n.toFin.isLt = n.toFin := rfl
+@[simp] theorem Fin.mk_uSizeToNat (n : USize) : Fin.mk n.toNat n.toFin.isLt = n.toFin := rfl
+
+@[simp] theorem BitVec.ofNatLT_uInt8ToNat (n : UInt8) : BitVec.ofNatLT n.toNat n.toFin.isLt = n.toBitVec := rfl
+@[simp] theorem BitVec.ofNatLT_uInt16ToNat (n : UInt16) : BitVec.ofNatLT n.toNat n.toFin.isLt = n.toBitVec := rfl
+@[simp] theorem BitVec.ofNatLT_uInt32ToNat (n : UInt32) : BitVec.ofNatLT n.toNat n.toFin.isLt = n.toBitVec := rfl
+@[simp] theorem BitVec.ofNatLT_uInt64ToNat (n : UInt64) : BitVec.ofNatLT n.toNat n.toFin.isLt = n.toBitVec := rfl
+@[simp] theorem BitVec.ofNatLT_uSizeToNat (n : USize) : BitVec.ofNatLT n.toNat n.toFin.isLt = n.toBitVec := rfl
+
+@[simp] theorem BitVec.ofFin_uInt8ToFin (n : UInt8) : BitVec.ofFin n.toFin = n.toBitVec := rfl
+@[simp] theorem BitVec.ofFin_uInt16ToFin (n : UInt16) : BitVec.ofFin n.toFin = n.toBitVec := rfl
+@[simp] theorem BitVec.ofFin_uInt32ToFin (n : UInt32) : BitVec.ofFin n.toFin = n.toBitVec := rfl
+@[simp] theorem BitVec.ofFin_uInt64ToFin (n : UInt64) : BitVec.ofFin n.toFin = n.toBitVec := rfl
+@[simp] theorem BitVec.ofFin_uSizeToFin (n : USize) : BitVec.ofFin n.toFin = n.toBitVec := rfl
+
+@[simp] theorem UInt8.toFin_toUInt16 (n : UInt8) : n.toUInt16.toFin = n.toFin.castLE (by decide) := rfl
+@[simp] theorem UInt8.toFin_toUInt32 (n : UInt8) : n.toUInt32.toFin = n.toFin.castLE (by decide) := rfl
+@[simp] theorem UInt8.toFin_toUInt64 (n : UInt8) : n.toUInt64.toFin = n.toFin.castLE (by decide) := rfl
+@[simp] theorem UInt8.toFin_toUSize (n : UInt8) :
+  n.toUSize.toFin = n.toFin.castLE size_le_usizeSize := rfl
+
+@[simp] theorem UInt16.toFin_toUInt32 (n : UInt16) : n.toUInt32.toFin = n.toFin.castLE (by decide) := rfl
+@[simp] theorem UInt16.toFin_toUInt64 (n : UInt16) : n.toUInt64.toFin = n.toFin.castLE (by decide) := rfl
+@[simp] theorem UInt16.toFin_toUSize (n : UInt16) :
+  n.toUSize.toFin = n.toFin.castLE size_le_usizeSize := rfl
+
+@[simp] theorem UInt32.toFin_toUInt64 (n : UInt32) : n.toUInt64.toFin = n.toFin.castLE (by decide) := rfl
+@[simp] theorem UInt32.toFin_toUSize (n : UInt32) :
+  n.toUSize.toFin = n.toFin.castLE size_le_usizeSize := rfl
+
+@[simp] theorem USize.toFin_toUInt64 (n : USize) : n.toUInt64.toFin = n.toFin.castLE size_le_usizeSize := rfl
+
+@[simp] theorem UInt16.toBitVec_toUInt8 (n : UInt16) : n.toUInt8.toBitVec = n.toBitVec.setWidth 8 := rfl
+@[simp] theorem UInt32.toBitVec_toUInt8 (n : UInt32) : n.toUInt8.toBitVec = n.toBitVec.setWidth 8 := rfl
+@[simp] theorem UInt64.toBitVec_toUInt8 (n : UInt64) : n.toUInt8.toBitVec = n.toBitVec.setWidth 8 := rfl
+@[simp] theorem USize.toBitVec_toUInt8 (n : USize) : n.toUInt8.toBitVec = n.toBitVec.setWidth 8 := BitVec.eq_of_toNat_eq (by simp)
+
+@[simp] theorem UInt8.toBitVec_toUInt16 (n : UInt8) : n.toUInt16.toBitVec = n.toBitVec.setWidth 16 := rfl
+@[simp] theorem UInt32.toBitVec_toUInt16 (n : UInt32) : n.toUInt16.toBitVec = n.toBitVec.setWidth 16 := rfl
+@[simp] theorem UInt64.toBitVec_toUInt16 (n : UInt64) : n.toUInt16.toBitVec = n.toBitVec.setWidth 16 := rfl
+@[simp] theorem USize.toBitVec_toUInt16 (n : USize) : n.toUInt16.toBitVec = n.toBitVec.setWidth 16 := BitVec.eq_of_toNat_eq (by simp)
+
+@[simp] theorem UInt8.toBitVec_toUInt32 (n : UInt8) : n.toUInt32.toBitVec = n.toBitVec.setWidth 32 := rfl
+@[simp] theorem UInt16.toBitVec_toUInt32 (n : UInt16) : n.toUInt32.toBitVec = n.toBitVec.setWidth 32 := rfl
+@[simp] theorem UInt64.toBitVec_toUInt32 (n : UInt64) : n.toUInt32.toBitVec = n.toBitVec.setWidth 32 := rfl
+@[simp] theorem USize.toBitVec_toUInt32 (n : USize) : n.toUInt32.toBitVec = n.toBitVec.setWidth 32 := BitVec.eq_of_toNat_eq (by simp)
+
+@[simp] theorem UInt8.toBitVec_toUInt64 (n : UInt8) : n.toUInt64.toBitVec = n.toBitVec.setWidth 64 := rfl
+@[simp] theorem UInt16.toBitVec_toUInt64 (n : UInt16) : n.toUInt64.toBitVec = n.toBitVec.setWidth 64 := rfl
+@[simp] theorem UInt32.toBitVec_toUInt64 (n : UInt32) : n.toUInt64.toBitVec = n.toBitVec.setWidth 64 := rfl
+@[simp] theorem USize.toBitVec_toUInt64 (n : USize) : n.toUInt64.toBitVec = n.toBitVec.setWidth 64 :=
+  BitVec.eq_of_toNat_eq (by simp [Nat.mod_eq_of_lt (USize.toNat_lt _)])
+
+@[simp] theorem UInt8.toBitVec_toUSize (n : UInt8) : n.toUSize.toBitVec = n.toBitVec.setWidth System.Platform.numBits :=
+  BitVec.eq_of_toNat_eq (by simp [Nat.mod_eq_of_lt n.toNat_lt_usizeSize])
+@[simp] theorem UInt16.toBitVec_toUSize (n : UInt16) : n.toUSize.toBitVec = n.toBitVec.setWidth System.Platform.numBits :=
+  BitVec.eq_of_toNat_eq (by simp [Nat.mod_eq_of_lt n.toNat_lt_usizeSize])
+@[simp] theorem UInt32.toBitVec_toUSize (n : UInt32) : n.toUSize.toBitVec = n.toBitVec.setWidth System.Platform.numBits :=
+  BitVec.eq_of_toNat_eq (by simp [Nat.mod_eq_of_lt n.toNat_lt_usizeSize])
+@[simp] theorem UInt64.toBitVec_toUSize (n : UInt64) : n.toUSize.toBitVec = n.toBitVec.setWidth System.Platform.numBits :=
+  BitVec.eq_of_toNat_eq (by simp)
+
+@[simp] theorem UInt8.ofNatLT_toNat (n : UInt8) : UInt8.ofNatLT n.toNat n.toNat_lt = n := rfl
+@[simp] theorem UInt16.ofNatLT_uInt8ToNat (n : UInt8) : UInt16.ofNatLT n.toNat (Nat.lt_trans n.toNat_lt (by decide)) = n.toUInt16 := rfl
+@[simp] theorem UInt32.ofNatLT_uInt8ToNat (n : UInt8) : UInt32.ofNatLT n.toNat (Nat.lt_trans n.toNat_lt (by decide)) = n.toUInt32 := rfl
+@[simp] theorem UInt64.ofNatLT_uInt8ToNat (n : UInt8) : UInt64.ofNatLT n.toNat (Nat.lt_trans n.toNat_lt (by decide)) = n.toUInt64 := rfl
+@[simp] theorem USize.ofNatLT_uInt8ToNat (n : UInt8) : USize.ofNatLT n.toNat n.toNat_lt_usizeSize = n.toUSize := rfl
+
+@[simp] theorem UInt16.ofNatLT_toNat (n : UInt16) : UInt16.ofNatLT n.toNat n.toNat_lt = n := rfl
+@[simp] theorem UInt32.ofNatLT_uInt16ToNat (n : UInt16) : UInt32.ofNatLT n.toNat (Nat.lt_trans n.toNat_lt (by decide)) = n.toUInt32 := rfl
+@[simp] theorem UInt64.ofNatLT_uInt16ToNat (n : UInt16) : UInt64.ofNatLT n.toNat (Nat.lt_trans n.toNat_lt (by decide)) = n.toUInt64 := rfl
+@[simp] theorem USize.ofNatLT_uInt16ToNat (n : UInt16) : USize.ofNatLT n.toNat n.toNat_lt_usizeSize = n.toUSize := rfl
+
+@[simp] theorem UInt32.ofNatLT_toNat (n : UInt32) : UInt32.ofNatLT n.toNat n.toNat_lt = n := rfl
+@[simp] theorem UInt64.ofNatLT_uInt32ToNat (n : UInt32) : UInt64.ofNatLT n.toNat (Nat.lt_trans n.toNat_lt (by decide)) = n.toUInt64 := rfl
+@[simp] theorem USize.ofNatLT_uInt32ToNat (n : UInt32) : USize.ofNatLT n.toNat n.toNat_lt_usizeSize = n.toUSize := rfl
+
+@[simp] theorem UInt64.ofNatLT_toNat (n : UInt64) : UInt64.ofNatLT n.toNat n.toNat_lt = n := rfl
+
+@[simp] theorem USize.ofNatLT_toNat (n : USize) : USize.ofNatLT n.toNat n.toNat_lt_size = n := rfl
+@[simp] theorem UInt64.ofNatLT_uSizeToNat (n : USize) : UInt64.ofNatLT n.toNat n.toNat_lt = n.toUInt64 := rfl
+
+-- We are not making these into `simp` lemmas because they lose the information stored in `h`. ·
+theorem UInt8.ofNatLT_uInt16ToNat (n : UInt16) (h) : UInt8.ofNatLT n.toNat h = n.toUInt8 :=
+  UInt8.toNat.inj (by simp [Nat.mod_eq_of_lt h])
+theorem UInt8.ofNatLT_uInt32ToNat (n : UInt32) (h) : UInt8.ofNatLT n.toNat h = n.toUInt8 :=
+  UInt8.toNat.inj (by simp [Nat.mod_eq_of_lt h])
+theorem UInt8.ofNatLT_uInt64ToNat (n : UInt64) (h) : UInt8.ofNatLT n.toNat h = n.toUInt8 :=
+  UInt8.toNat.inj (by simp [Nat.mod_eq_of_lt h])
+theorem UInt8.ofNatLT_uSizeToNat (n : USize) (h) : UInt8.ofNatLT n.toNat h = n.toUInt8 :=
+  UInt8.toNat.inj (by simp [Nat.mod_eq_of_lt h])
+theorem UInt16.ofNatLT_uInt32ToNat (n : UInt32) (h) : UInt16.ofNatLT n.toNat h = n.toUInt16 :=
+  UInt16.toNat.inj (by simp [Nat.mod_eq_of_lt h])
+theorem UInt16.ofNatLT_uInt64ToNat (n : UInt64) (h) : UInt16.ofNatLT n.toNat h = n.toUInt16 :=
+  UInt16.toNat.inj (by simp [Nat.mod_eq_of_lt h])
+theorem UInt16.ofNatLT_uSizeToNat (n : USize) (h) : UInt16.ofNatLT n.toNat h = n.toUInt16 :=
+  UInt16.toNat.inj (by simp [Nat.mod_eq_of_lt h])
+theorem UInt32.ofNatLT_uInt64ToNat (n : UInt64) (h) : UInt32.ofNatLT n.toNat h = n.toUInt32 :=
+  UInt32.toNat.inj (by simp [Nat.mod_eq_of_lt h])
+theorem UInt32.ofNatLT_uSizeToNat (n : USize) (h) : UInt32.ofNatLT n.toNat h = n.toUInt32 :=
+  UInt32.toNat.inj (by simp [Nat.mod_eq_of_lt h])
+theorem USize.ofNatLT_uInt64ToNat (n : UInt64) (h) : USize.ofNatLT n.toNat h = n.toUSize :=
+  USize.toNat.inj (by simp [Nat.mod_eq_of_lt h])
+
+@[simp] theorem UInt8.ofFin_toFin (n : UInt8) : UInt8.ofFin n.toFin = n := rfl
+@[simp] theorem UInt16.ofFin_toFin (n : UInt16) : UInt16.ofFin n.toFin = n := rfl
+@[simp] theorem UInt32.ofFin_toFin (n : UInt32) : UInt32.ofFin n.toFin = n := rfl
+@[simp] theorem UInt64.ofFin_toFin (n : UInt64) : UInt64.ofFin n.toFin = n := rfl
+@[simp] theorem USize.ofFin_toFin (n : USize) : USize.ofFin n.toFin = n := rfl
+
+@[simp] theorem UInt16.ofFin_uint8ToFin (n : UInt8) : UInt16.ofFin (n.toFin.castLE (by decide)) = n.toUInt16 := rfl
+
+@[simp] theorem UInt32.ofFin_uint8ToFin (n : UInt8) : UInt32.ofFin (n.toFin.castLE (by decide)) = n.toUInt32 := rfl
+@[simp] theorem UInt32.ofFin_uint16ToFin (n : UInt16) : UInt32.ofFin (n.toFin.castLE (by decide)) = n.toUInt32 := rfl
+
+@[simp] theorem UInt64.ofFin_uint8ToFin (n : UInt8) : UInt64.ofFin (n.toFin.castLE (by decide)) = n.toUInt64 := rfl
+@[simp] theorem UInt64.ofFin_uint16ToFin (n : UInt16) : UInt64.ofFin (n.toFin.castLE (by decide)) = n.toUInt64 := rfl
+@[simp] theorem UInt64.ofFin_uint32ToFin (n : UInt32) : UInt64.ofFin (n.toFin.castLE (by decide)) = n.toUInt64 := rfl
+
+@[simp] theorem USize.ofFin_uint8ToFin (n : UInt8) : USize.ofFin (n.toFin.castLE UInt8.size_le_usizeSize) = n.toUSize := rfl
+@[simp] theorem USize.ofFin_uint16ToFin (n : UInt16) : USize.ofFin (n.toFin.castLE UInt16.size_le_usizeSize) = n.toUSize := rfl
+@[simp] theorem USize.ofFin_uint32ToFin (n : UInt32) : USize.ofFin (n.toFin.castLE UInt32.size_le_usizeSize) = n.toUSize := rfl
