src/Init/Prelude.lean
@@ -2150,14 +2150,14 @@ instance : Inhabited UInt64 where
 /-- The size of type `USize`, that is, `2^System.Platform.numBits`. -/
 abbrev USize.size : Nat := (hPow 2 System.Platform.numBits)
 
-theorem usize_size_eq : Or (Eq USize.size 4294967296) (Eq USize.size 18446744073709551616) :=
+theorem USize.size_eq : Or (Eq USize.size 4294967296) (Eq USize.size 18446744073709551616) :=
   show Or (Eq (hPow 2 System.Platform.numBits) 4294967296) (Eq (hPow 2 System.Platform.numBits) 18446744073709551616) from
   match System.Platform.numBits, System.Platform.numBits_eq with
   | _, Or.inl rfl => Or.inl (of_decide_eq_true rfl)
   | _, Or.inr rfl => Or.inr (of_decide_eq_true rfl)
 
-theorem usize_size_pos : LT.lt 0 USize.size :=
-  match USize.size, usize_size_eq with
+theorem USize.size_pos : LT.lt 0 USize.size :=
+  match USize.size, USize.size_eq with
   | _, Or.inl rfl => of_decide_eq_true rfl
   | _, Or.inr rfl => of_decide_eq_true rfl
 
@@ -2207,7 +2207,7 @@ def USize.decEq (a b : USize) : Decidable (Eq a b) :=
 instance : DecidableEq USize := USize.decEq
 
 instance : Inhabited USize where
-  default := USize.ofNatLT 0 usize_size_pos
+  default := USize.ofNatLT 0 USize.size_pos
 
 /--
 A `Nat` denotes a valid unicode codepoint if it is less than `0x110000`, and
